rest consistency

Foundation/Modal/Kripke2/FiniteFrame.lean
@@ -105,14 +105,62 @@ class FiniteDefinedBy (C Γ) extends FiniteFrameClass.DefinedBy C Γ where
 
 abbrev DefinedByFormula (C) (φ : Formula ℕ) := FiniteFrameClass.DefinedBy C {φ}
 
+lemma definedByFormula_of_iff_mem_validate (h : ∀ F, F ∈ C ↔ F ⊧ φ) : DefinedByFormula C φ := by
+  constructor;
+  simpa;
+
+instance definedBy_inter
+  (C₁ Γ₁) [h₁ : DefinedBy C₁ Γ₁]
+  (C₂ Γ₂) [h₂ : DefinedBy C₂ Γ₂]
+  : DefinedBy (C₁ ∩ C₂) (Γ₁ ∪ Γ₂) := ⟨by
+  rintro F;
+  constructor
+  . rintro ⟨hF₁, hF₂⟩;
+    rintro φ (hφ₁ | hφ₂);
+    . exact h₁.defines F |>.mp hF₁ _ hφ₁;
+    . exact h₂.defines F |>.mp hF₂ _ hφ₂;
+  . intro h;
+    constructor;
+    . apply h₁.defines F |>.mpr;
+      intro φ hφ;
+      apply h;
+      left;
+      assumption;
+    . apply h₂.defines F |>.mpr;
+      intro φ hφ;
+      apply h;
+      right;
+      assumption;
+⟩
+
 class IsNonempty (C : Kripke.FiniteFrameClass) where
   nonempty : Nonempty C
 
 end FiniteFrameClass
 
 
-abbrev AllFiniteFrameClass : FrameClass := Set.univ
+abbrev AllFiniteFrameClass : FiniteFrameClass := Set.univ
 
+instance AllFiniteFrameClass.DefinedBy : AllFiniteFrameClass.DefinedByFormula (Axioms.K (.atom 0) (.atom 1)) :=
+  FiniteFrameClass.definedByFormula_of_iff_mem_validate $ by
+    simp only [Set.mem_univ, true_iff];
+    intro F;
+    exact Formula.Kripke.ValidOnFrame.axiomK;
+
+instance AllFiniteFrameClass.IsNonempty : AllFiniteFrameClass.IsNonempty := by
+  use ⟨Unit, λ _ _ => True⟩;
+  simp;
+
+
+namespace FiniteFrameClass
+
+variable {C : Kripke.FiniteFrameClass}
+
+instance definedBy_with_axiomK (defines : C.DefinedBy Γ) : DefinedBy C (insert (Axioms.K (.atom 0) (.atom 1)) Γ) := by
+  convert FiniteFrameClass.definedBy_inter AllFiniteFrameClass {Axioms.K (.atom 0) (.atom 1)} C Γ
+  simp;
+
+end FiniteFrameClass
 
 end Kripke
 
