Foundation.lean
@@ -129,4 +129,4 @@ import Foundation.Modal.Kripke2.NNFormula
 import Foundation.Modal.Kripke2.ComplexityLimited
 import Foundation.Modal.Kripke2.Undefinability
 
-import Foundation.Modal.PLoN.N
+import Foundation.Modal.PLoN.Hilbert.N
